Cleanup and documentation for the closure conversion proof at closure_conversion_correct.v

theories/L6_PCPS/closure_conversion_correct.v
@@ -9,10 +9,36 @@ Import ListNotations.
 Open Scope ctx_scope.
 
 
-(* It should be the case that variables in FV are
- * shadowed by variables with the same name in xs *)
+(** For closure conversion, the free variables of an expression are divided in
+    three categories :
 
-(** Invariant about closure environments. *)
+    1. Variables in the current scope, i.e. arguments of the current function
+    and bindings in the body of the current function definition.
+
+    2. Names of the functions that are defined in the current block of mutually
+    recursive functions.
+
+    3. Free variables, i.e. variables that are not declared outside of the
+    body of the current function but in outer definitions
+
+    In the proof maintains different invariants for each kind of variable *)
+
+
+(** * Invariants *)
+
+(** Naming conventions in the following :
+
+    [Scope] : The set of variables in the current scope.
+
+    [Funs] : The set of variables in the current block of mutually recursive
+    functions.
+
+    [FVs] : The list of free variables (needs to be ordered).
+
+    [Γ] : The formal parameter of the environment after closure conversion. *)
+
+
+(** Invariant about the values of free variables. *)
 Definition closure_env k rho Scope Funs vs FVs : Prop :=
   forall (x : var) N (v : val),
     ~ In _ Scope x ->
@@ -23,7 +49,7 @@ Definition closure_env k rho Scope Funs vs FVs : Prop :=
                    cc_approx_val k v v'.
 
 (** Invariant about the free variables *) 
-Definition env_inv k rho rho' Scope Funs Γ FVs : Prop :=
+Definition FV_inv k rho rho' Scope Funs Γ FVs : Prop :=
   exists tau t vs,
     M.get Γ rho' = Some (Vconstr tau t vs) /\
     closure_env k rho Scope Funs vs FVs.
@@ -42,40 +68,17 @@ Definition Fun_inv k (rho rho' : env) Scope Funs Γ : Prop :=
         cc_approx_val k (Vfun rho1 B1 f1)
                       (Vconstr tau' t' [(Vfun rho2 B2 f2) ; (Vconstr tau t vs)]).
 
-(* XXX : deprecated *)
-Lemma Fun_inv_extend' k rho rho' Scope Funs Γ
-      f rho1 B1 f1 rho2 B2 f2 tau t vs:
-  Fun_inv k rho (M.set Γ (Vconstr tau t vs) rho') Scope Funs Γ ->
-  f <> Γ ->
-  (exists tau' t',
-     cc_approx_val k (Vfun rho1 B1 f1)
-                   (Vconstr tau' t' [(Vfun rho2 B2 f2) ; (Vconstr tau t vs)])) ->
-  Fun_inv k (M.set f (Vfun rho1 B1 f1) rho)
-          (M.set Γ (Vconstr tau t vs) (M.set f  (Vfun rho2 B2 f2) rho'))
-          Scope (Union _ (Singleton _ f) Funs) Γ.
-Proof.
-  intros Hinv Hneq Hv. edestruct Hinv as [tau' [t' [vs' [Hget Hyp]]]].
-  rewrite M.gss in Hget. inv Hget.
-  do 3 eexists. rewrite M.gss. split; [ reflexivity |].
-  intros f' v Hnin Hin Hget'.
-  rewrite M.gsspec in Hget'. destruct (Coqlib.peq f' f); subst.
-  - inv Hget'.
-    edestruct Hv as [tau1 [t1 Happrox]]; eauto.
-    repeat eexists. rewrite M.gso; eauto. now rewrite M.gss; eauto.
-    eassumption.
-  - edestruct Hyp as
-        [rho3 [B3 [f3 [rho4 [B4 [f4 [tau2 [t2 [Heq [Hget2 Happrox]]]]]]]]]];
-    subst; eauto.
-    + inv Hin; eauto. inv H. congruence.
-    + repeat eexists; eauto.
-      rewrite M.gsspec in Hget2.
-      destruct (Coqlib.peq f' Γ); subst.
-      * inv Hget2.
-      * do 2 (rewrite M.gso; eauto).
-Qed.
 
-Lemma Fun_inv_extend k rho rho' Scope Funs Γ
-      f rho1 B1 f1 rho2 B2 f2 tau t vs:
+(** The variables in S are defined in the environment. Will be used to state
+    that the free variables of an expression are present in the environment *)
+Definition vars_in_env S (rho : env) : Prop :=
+  forall x, In _ S x -> exists v, M.get x rho = Some v. 
+
+(** * Lemmas about Fun_inv *)
+
+(** Extend the two environments with a variable that is not the current environment
+    arguments (i.e. [Γ]) *)
+Lemma Fun_inv_set k rho rho' Scope Funs Γ f rho1 B1 f1 rho2 B2 f2 tau t vs:
   Fun_inv k rho rho' Scope Funs Γ ->
   f <> Γ ->
   M.get Γ rho' = Some (Vconstr tau t vs) ->
@@ -98,40 +101,10 @@ Proof.
         [rho3 [B3 [f3 [rho4 [B4 [f4 [tau2 [t2 [Heq [Hget2 Happrox]]]]]]]]]];
     subst; eauto.
     + inv Hin; eauto. inv H. congruence.
-    + repeat eexists; eauto.
-      rewrite M.gso; eauto.
+    + repeat eexists; eauto. rewrite M.gso; eauto.
 Qed.
 
-Lemma closure_conversion_fundefs_find_def Funs FVs B1 B2 f t1 xs e1 :
-  Closure_conversion_fundefs Funs FVs B1 B2 ->
-  find_def f B1 = Some (t1, xs, e1) ->
-  exists t2 Γ' e2,
-    ~ In var (Union var Funs (Union _ (FromList xs) (bound_var e1))) Γ' /\
-    find_def f B2 = Some (t2, Γ' :: xs, e2) /\
-    Closure_conversion (FromList xs) Funs Γ' FVs e1 e2.
-Proof.
-  intros Hcc Hdef. induction Hcc.
-  - simpl in Hdef. destruct (M.elt_eq f f0) eqn:Heq; subst.
-    + inv Hdef. repeat eexists; eauto.
-      simpl. rewrite Heq. reflexivity.
-    + edestruct IHHcc as [t2 [Γ'' [e2 [Hnin [Hfind Hcc']]]]]; eauto.
-      repeat eexists; eauto. simpl; rewrite Heq. eassumption.
-  - inv Hdef.
-Qed.
-
-Lemma cc_approx_env_P_set_not_in_P_r
-      (x : var) (v : val) (P : Ensemble var) (k : nat) (rho1 rho2 : env):
-  cc_approx_env_P P k rho1 rho2 ->
-  Disjoint var P (Singleton var x) -> cc_approx_env_P P k rho1 (M.set x v rho2).
-Proof.
-  intros Hcc HD y HP v' Hget.
-  edestruct (Coqlib.peq x y); subst.
-  - exfalso. eapply HD; eauto.
-  - edestruct Hcc as [v2 [Hget' Hcc']]; eauto.
-    eexists. rewrite M.gso. split; eauto.
-    congruence.
-Qed.
-
+(** Rename the environment parameter *)
 Lemma Fun_inv_rename k rho1 rho2 Scope Funs Γ Γ' v :
   ~ In _ Funs Γ ->  ~ In _ Funs Γ' ->
   Fun_inv k rho1 (M.set Γ v rho2) Scope Funs Γ ->
@@ -149,6 +122,7 @@ Proof.
   repeat eexists; eauto. rewrite M.gso; eauto.
 Qed.
 
+(** [Fun_inv] is monotonic on its 3rd argument *)
 Lemma Fun_inv_mon k rho1 rho2 Scope Scope' Funs Γ :
   Included _ Scope Scope' -> 
   Fun_inv k rho1 rho2 Scope Funs Γ ->
@@ -160,6 +134,7 @@ Proof.
   now eapply H; eauto. 
 Qed.
 
+(** Extend the first environment with a variable in [Scope] *)
 Lemma Fun_inv_set_In_Scope_l k rho1 rho2 Scope Funs Γ x v :
   In _ Scope x ->
   Fun_inv k rho1 rho2 Scope Funs Γ ->
@@ -173,6 +148,7 @@ Proof.
   edestruct H as [v'' [tau' [t' [Hget'' Happrox']]]]; eauto.
 Qed.
 
+(** Extend the second environment with a variable in [Scope] *)
 Lemma Fun_inv_set_In_Scope_r k rho1 rho2 Scope Funs Γ x v v' :
   In _ Scope x ->
   Fun_inv k rho1 (M.set Γ v rho2) Scope Funs Γ ->
@@ -193,6 +169,8 @@ Proof.
     rewrite M.gso; eauto. eassumption.
 Qed.
 
+(** Extend the second environment with a variable in [Scope] that is different
+    from [Γ] *)
 Lemma Fun_inv_set_In_Scope_r_not_Γ k rho1 rho2 Scope Funs Γ x v :
   In _ Scope x ->
   x <> Γ ->
@@ -209,6 +187,9 @@ Proof.
   do 8 eexists. rewrite M.gso; eauto.
 Qed.
 
+
+(** Extend the second environment with a variable not in [Funs] that is different
+    from Γ *)
 Lemma Fun_inv_set_not_In_Funs_r_not_Γ k rho1 rho2 Scope Funs Γ x v :
   ~ In _ Funs x ->
   x <> Γ ->
@@ -225,7 +206,7 @@ Proof.
   do 8 eexists. rewrite M.gso; eauto.
 Qed.
 
-
+(** Extend the first environment with a list of variables in [Scope] *)
 Lemma Fun_inv_setlist_In_Scope_l k rho1 rho1' rho2 Scope Funs Γ xs vs :
   Included _ (FromList xs) Scope ->
   Fun_inv k rho1 rho2 Scope Funs Γ ->
@@ -248,6 +229,7 @@ Proof.
       eapply Included_Union_r.
 Qed.
 
+(** Extend the second environment with a list of variables in [Scope] *)
 Lemma Fun_inv_setlist_In_Scope_r k rho1 rho2 rho2' Scope Funs Γ xs vs v :
   Included _ (FromList xs) Scope ->
   Fun_inv k rho1 (M.set Γ v rho2) Scope Funs Γ ->
@@ -269,17 +251,7 @@ Proof.
       eapply Included_Union_r.
 Qed.
 
-Lemma Closure_conversion_fundefs_name_in_fundefs Funs FVs B1 B2  :
-  Closure_conversion_fundefs Funs FVs B1 B2 ->
-  Same_set _ (name_in_fundefs B1) (name_in_fundefs B2).
-Proof.
-  intros Hcc. induction Hcc; simpl.
-  - eapply Same_set_Union_compat.
-    now eapply Same_set_refl.
-    now eauto.
-  - now apply Same_set_refl.
-Qed.
-
+(** Redefine the environment argument in the second environment *)
 Lemma Fun_inv_reset k rho rho' B v Scope Funs Γ :
   ~ In _ (name_in_fundefs B) Γ ->
   Fun_inv k rho
@@ -311,66 +283,161 @@ Proof.
       intros Hc; subst; eauto.
 Qed.
 
-Lemma get_def_funs_In_names B' B f rho :
-  In var (name_in_fundefs B) f ->
-  exists v : val, M.get f (def_funs B' B rho rho) = Some v.
+Instance Fun_inv_proper :
+  Proper (Logic.eq ==> Logic.eq ==> Logic.eq ==> Same_set var ==> Logic.eq ==> Logic.eq ==> iff)
+         (Fun_inv).
 Proof.
-  induction B; intros Hin; inv Hin. 
-  - inv H. eexists. simpl. rewrite M.gss. eauto.
-  - edestruct IHB as [v' Heq]; eauto.
-    destruct (Coqlib.peq f v) eqn:Heq'.
-    + eexists. simpl. now rewrite M.gsspec, Heq'.
-    + eexists. simpl. rewrite M.gsspec, Heq'.
-      eassumption.
+  constructor; subst; intros [tau [t [vs [Hget Hfun]]]];
+  do 3 eexists; split; eauto;
+  intros; eapply Hfun; eauto; intros Hc; eapply H; eapply H2; eauto.
 Qed.
 
-Lemma get_setlist_In_xs x xs vs rho rho' :
-  In var (FromList xs) x ->
-  setlist xs vs rho = Some rho' ->
-  exists v : val, M.get x rho' = Some v.
+(** Define a block of functions in the first environment and put the in the
+    current scope *)
+Lemma Fun_inv_def_funs_l k rho rho' B1 B1' Scope Funs Γ:
+  Fun_inv k rho rho' Scope Funs Γ ->
+  Fun_inv k (def_funs B1 B1' rho rho) rho'
+          (Union _ (name_in_fundefs B1')  Scope) Funs Γ.
 Proof.
-  revert rho rho' vs. induction xs; intros rho rho' vs Hin Hset.
-  - rewrite FromList_nil in Hin. exfalso.
-    eapply not_In_Empty_set. eassumption. 
-  - rewrite FromList_cons in Hin.
-    destruct vs; try discriminate.    
-    simpl in Hset. destruct (setlist xs vs rho) eqn:Hsetlist; try discriminate.
-    inv Hset. inv Hin.
-    + inv H. eexists. rewrite M.gss. reflexivity.
-    + destruct (Coqlib.peq x a); subst.
-      * eexists. now rewrite M.gss.
-      * edestruct IHxs; eauto.
-        eexists. simpl. rewrite M.gso; eauto. 
+  intros [t [tau [v [Hget Hfun]]]].
+  do 3 eexists. split; eauto.
+  intros f v' Hnin Hin Hget'.
+  rewrite def_funs_neq in Hget'; eauto.
 Qed.
 
-Definition vars_in_env S (rho : env) : Prop :=
-  forall x, In _ S x -> exists v, M.get x rho = Some v. 
+(** Define a block of functions in the second environment and put the in the
+    current scope *)
+Lemma Fun_inv_def_funs_r k rho rho' B1 B1' Scope Funs Γ:
+  ~ In _ (name_in_fundefs B1') Γ ->
+  Fun_inv k rho rho' Scope Funs Γ ->
+  Fun_inv k rho (def_funs B1 B1' rho' rho')
+          (Union _ (name_in_fundefs B1') Scope) Funs Γ.
+Proof.
+  intros Hin [t [tau [v [Hget Hfun]]]].
+  do 3 eexists. split; eauto. 
+  rewrite def_funs_neq; eauto.
+  intros f v' Hnin Hin' Hget'.
+  edestruct Hfun as
+      [rho1' [B2 [f1 [rho2' [B2' [f2 [tau2 [t2 [Heq' [Hget2 Happrox2]]]]]]]]]]; eauto.
+  repeat eexists; eauto.
+  rewrite def_funs_neq; eauto.
+Qed.
 
-Inductive unique_functions : fundefs -> Prop :=
-| Fnil_un :
-    unique_functions Fnil
-| Fcons_un :
-    forall f tau xs e B,
-      unique_functions B ->
-      ~ In _ (name_in_fundefs B) f ->
-      unique_functions (Fcons f tau xs e B).
+(** Define a block of functions in both environments and put the in the
+    current scope *)
+Lemma Fun_inv_def_funs k rho rho' B1 B1' B2 B2' Scope Funs Γ:
+  ~ In _ (name_in_fundefs B1') Γ ->
+  Same_set _ (name_in_fundefs B1') (name_in_fundefs B2') ->
+  Fun_inv k rho rho' Scope Funs Γ ->
+  Fun_inv k  (def_funs B1 B1' rho rho) (def_funs B2 B2' rho' rho')
+          (Union _ (name_in_fundefs B1') Scope) Funs Γ.
+Proof.
+  intros Hin HS [t [tau [v [Hget Hfun]]]].
+  do 3 eexists. split; eauto. 
+  rewrite def_funs_neq; eauto.
+  intros Hc. eapply Hin. now eapply HS.
+  intros f v' Hnin Hin' Hget'.
+  rewrite def_funs_neq in Hget'; eauto.
+  edestruct Hfun as
+      [rho1' [B3 [f1 [rho2' [B3' [f2 [tau2 [t2 [Heq' [Hget2 Happrox2]]]]]]]]]]; eauto.
+  repeat eexists; eauto.
+  rewrite def_funs_neq; eauto.
+  intros Hc. eapply Hnin. left. now rewrite HS.
+Qed.
 
-Definition fundefs_names_unique (e : exp) : Prop :=
-  forall B, funs_in_exp B e -> unique_functions B.
+(** * Lemmas about FV_inv *)
 
-Definition fundefs_names_unique_fundefs (B : fundefs) : Prop :=
-  forall B', funs_in_fundef B' B \/ B' = B -> unique_functions B'.
+(** Extend the first environment with a variable in [Scope] *)
+Lemma FV_inv_set_In_Scope_l k rho rho' x v Scope Funs FVs Γ :
+  In var Scope x ->
+  FV_inv k rho rho' Scope Funs Γ FVs ->
+  FV_inv k (M.set x v rho) rho' Scope Funs Γ FVs.
+Proof.
+  intros Hin HInv. destruct HInv as [tau [t  [vs [Hget H]]]].
+  do 3 eexists; split; eauto. intros y n v' Hnin Hnin' Hnth Hget'.
+  rewrite M.gsspec in Hget'. destruct (Coqlib.peq y x); subst.
+  - contradiction. 
+  - eauto. 
+Qed.
 
+(** Extend the second environment with a variable in [Scope] that is not [Γ].
+    XXX : deprecated. See [FV_inv_set_r] *)
+Lemma FV_inv_set_In_Scope_r k rho rho' x v Scope Funs FVs Γ :
+  In var Scope x ->
+  x <> Γ ->
+  FV_inv k rho rho' Scope Funs Γ FVs ->
+  FV_inv k rho (M.set x v rho') Scope Funs Γ FVs.
+Proof.
+  intros Hin Hneq HInv. destruct HInv as [tau [t  [vs [Hget H]]]].
+  do 3 eexists; split; eauto. rewrite M.gso; eauto.
+Qed.
+
+(** Extend the first environment with a variable not in [FVs] *)
+Lemma FV_inv_set_not_In_FVs_l k rho rho' x v Scope Funs Γ FVs :
+  ~ List.In x FVs ->
+  FV_inv k rho rho' Scope Funs Γ FVs ->
+  FV_inv k (M.set x v rho) rho' Scope Funs Γ FVs.
+Proof.
+  intros Hin HInv. destruct HInv as [tau [t  [vs [Hget H]]]].
+  do 3 eexists; split; eauto. intros y n v' Hnin Hnin' Hnth Hget'.
+  rewrite M.gsspec in Hget'. destruct (Coqlib.peq y x); subst.
+  - inv Hget. eapply H; eauto.
+    eapply nthN_In in Hnth.
+    contradiction.
+  - eauto.
+Qed.
+
+(** Extend the second environment with a variable that is not [Γ] *)
+Lemma FV_inv_set_r k rho rho' x v Scope Funs Γ FVs :
+  x <> Γ ->
+  FV_inv k rho rho' Scope Funs Γ FVs ->
+  FV_inv k rho (M.set x v rho') Scope Funs Γ FVs.
+Proof.
+  intros Hin HInv. destruct HInv as [tau [t  [vs [Hget H]]]].
+  do 3 eexists; split; eauto. 
+  rewrite M.gso; eauto. 
+Qed.
+
+(** Extend the [Scope]. TODO : replace with monotonicity property? *)
+Lemma FV_inv_extend_Scope k rho rho' Scope Funs Γ FVs x :
+  FV_inv k rho rho' Scope Funs Γ FVs ->
+  FV_inv k rho rho' (Union _ (Singleton _ x) Scope) Funs Γ FVs.
+Proof.
+  intros [tau [t  [vs [Hget H]]]].
+  do 3 eexists; split; eauto. 
+  intros y N v Hnin Hnin' Hnth Hget'. eapply H; eauto.
+Qed.
+
+(** Define a block of functions in both environments and put the in the
+    current scope *)
+Lemma FV_inv_def_funs k rho rho' B1 B1' B2 B2' Scope Funs Γ FVs:
+  ~ In _ (name_in_fundefs B1') Γ ->
+  Same_set _ (name_in_fundefs B1') (name_in_fundefs B2') ->
+  FV_inv k rho rho' Scope Funs Γ FVs ->
+  FV_inv k  (def_funs B1 B1' rho rho) (def_funs B2 B2' rho' rho')
+          (Union _ (name_in_fundefs B1') Scope) Funs Γ FVs.
+Proof.
+  intros Hin HS [t [tau [v [Hget Henv]]]].
+  do 3 eexists. split; eauto. 
+  rewrite def_funs_neq; eauto.
+  intros Hc. eapply Hin. now eapply HS.
+  intros f N v' Hnin Hnin' Hnth Hget'.
+  rewrite def_funs_neq in Hget'; eauto.
+Qed.
+
+(** * Lemmas about [vars_in_env] *)
+
+(** [vars_in_env] is anti-monotonic on its first argument *)
 Lemma vars_in_env_antimon S S' rho :
   Included _ S' S ->
   vars_in_env S rho ->
   vars_in_env S' rho.
 Proof.
   intros Hin Hv x Hs. eauto.
-
 Qed.
 
-Lemma vars_in_env_extend x v S rho :
+(** Extend the environment with a variable and put it in the set *)
+Lemma vars_in_env_set x v S rho :
   vars_in_env S rho ->
   vars_in_env (Union _ S (Singleton _ x)) (M.set x v rho).
 Proof. 
@@ -383,17 +450,7 @@ Proof.
   - inv H0. eexists. rewrite M.gss. eauto.
 Qed.
 
-Instance Decidable_FromList (l : list var) : Decidable (FromList l). 
-Proof. 
-  constructor. intros x. induction l. 
-  - right. intros H. inv H. 
-  - destruct (Coqlib.peq a x).
-    + subst. left. constructor. eauto.
-    + destruct IHl. left. now constructor 2.
-      right. intros Hc. eapply H. inv Hc; eauto.
-      congruence.
-Qed.
-
+(** Extend the environment with a list of variables and put them in the set *)
 Lemma vars_in_env_setlist xs vs S rho rho' :
   vars_in_env S rho ->
   setlist xs vs rho = Some rho' ->
@@ -407,238 +464,21 @@ Proof.
     eexists. erewrite <- setlist_not_In; eauto.
 Qed.
 
+(** Extend the environment with a block of functions and put them in the set *)
 Lemma vars_in_env_def_funs B' B rho S  :
   vars_in_env S rho ->
   vars_in_env (Union _ (name_in_fundefs B) S) (def_funs B' B rho rho).
 Proof.
   intros H x' Hs.
   destruct (Decidable_name_in_fundefs B). destruct (Dec x').
-  - eapply get_def_funs_In_names; eauto.
+  - eexists. rewrite def_funs_eq; eauto.
   - destruct Hs; try contradiction. 
     edestruct H; eauto.
     eexists. erewrite def_funs_neq; eauto.
 Qed.
 
-Lemma closure_conversion_fundefs_correct k rho rho' B1 B2 B1' B2'
-      Scope Γ FVs Funs' FVs' t tau vs:
-  (* The IH *)
-  (forall m : nat,
-     m < k ->
-     forall (e : exp) (rho rho' : env) (e' : exp)
-       (Scope Funs : Ensemble var) (Γ : var) (FVs : list M.elt),
-       cc_approx_env_P Scope m rho rho' ->
-       ~ In var (bound_var e) Γ ->
-       vars_in_env (occurs_free e) rho ->
-       fundefs_names_unique e ->
-       Fun_inv m rho rho' Scope Funs Γ ->
-       env_inv m rho rho' Scope Funs Γ FVs ->
-       Closure_conversion Scope Funs Γ FVs e e' ->
-       cc_approx_exp m (e, rho) (e', rho')) ->
-  Same_set _ (occurs_free_fundefs B1) (FromList FVs) ->
-  fundefs_names_unique_fundefs B1 ->
-  vars_in_env (occurs_free_fundefs B1) rho ->
-  Closure_conversion_fundefs (name_in_fundefs B1) FVs B1 B2 ->
-  Closure_conversion_fundefs Funs' FVs' B1' B2' ->
-  ~ In _ (name_in_fundefs B1) Γ ->
-  ~ In _ (name_in_fundefs B1') Γ ->
-  closure_env k rho (Empty_set _) (Empty_set _) vs FVs ->
-  Fun_inv k (def_funs B1 B1' rho rho)
-          (def_funs B2 B2' (M.set Γ (Vconstr tau t vs) rho') (M.set Γ (Vconstr tau t vs) rho'))
-          Scope (name_in_fundefs B1') Γ.
-Proof.
-  revert B1' rho rho' B2 B1 B2' Scope Γ FVs Funs' FVs' t tau vs.
-  induction k as [k IHk] using lt_wf_rec1.
-  induction B1'; 
-    intros rho rho' B2 B1 B2' Scope Γ FVs Funs' FVs' t' tau' vs
-           IHe Hs Hun Hfv Hcc Hcc' Hnin Hnin' Henv.
-  - inv Hcc'. simpl.
-    eapply Fun_inv_extend.
-    + eapply IHB1'; eauto.
-      intros Hc. apply Hnin'.
-      simpl; eauto.
-    + intros Hc. apply Hnin'. subst. simpl; eauto.
-    + rewrite def_funs_neq.
-      rewrite M.gss. reflexivity.
-      simpl in Hnin'.
-      rewrite Closure_conversion_fundefs_name_in_fundefs in Hnin';
-        [now eauto | eassumption ].
-    + exists tau', t.
-      rewrite cc_approx_val_eq.
-      intros vs1 vs2 j t1 xs1 e1 rho1' Hlen Hfind Hset.
-      edestruct setlist_length
-      with (rho' := def_funs B2 B2 (M.set Γ (Vconstr tau' t' vs) rho')
-                             (M.set Γ (Vconstr tau' t' vs) rho')) as [rho2' Hset'].
-      eassumption. now eauto.
-      edestruct closure_conversion_fundefs_find_def
-        as [t2 [Γ'' [e2 [Hnin'' [Hfind' Hcc']]]]]; [| eassumption |]. eassumption.
-      exists t2, Γ'', xs1. do 2 eexists.
-      split. eassumption. split.
-      simpl. rewrite Hset'. reflexivity.
-      intros Hlt Hall.  
-      eapply IHe; try eassumption.  
-      * eapply cc_approx_env_P_set_not_in_P_r.
-        eapply cc_approx_env_P_setlist_l with (P1 := Empty_set _); eauto. 
-        eapply cc_approx_env_Empty_set.
-        intros x H1 H2. contradiction.
-        constructor. intros x Hc. inv Hc. inv H0. eauto.
-      * intros Hc. apply Hnin''. eauto.
-      * eapply vars_in_env_antimon.
-        eapply occurs_free_in_fun. eapply find_def_correct. eassumption.
-        eapply vars_in_env_setlist; [| now eauto ].
-        eapply vars_in_env_def_funs. eassumption.
-      * intros B Hin. eapply Hun. left. 
-        eapply fun_in_fundefs_funs_in_fundef; eauto.
-        eapply find_def_correct. eassumption.
-      * assert
-          (Fun_inv j (def_funs B1 B1 rho rho)
-                   (def_funs B2 B2 (M.set Γ (Vconstr tau' t' vs) rho')
-                             (M.set Γ (Vconstr tau' t' vs) rho'))
-                   (FromList xs1) (name_in_fundefs B1) Γ).
-        { eapply IHk; try eassumption.
-          - intros. eapply IHe; eauto. omega. 
-          - intros x1 N v1 Hnin1 Hnin2 Hnth Hget.
-            edestruct Henv as [v2 [Hnth' Happ']]; eauto.
-            eexists; split; eauto. eapply cc_approx_val_monotonic.
-            eassumption. omega. } 
-        eapply Fun_inv_rename with (Γ := Γ); eauto.
-        eapply Fun_inv_setlist_In_Scope_l; [ now apply Included_refl | |].
-        eapply Fun_inv_setlist_In_Scope_r; [ now apply Included_refl | |]. 
-        eapply Fun_inv_reset; [| eassumption ].
-        rewrite <- Closure_conversion_fundefs_name_in_fundefs; [ | eassumption ].
-        now eauto. now eauto. now eauto.
-      * do 3 eexists. split.
-        rewrite M.gss. reflexivity.
-        intros x N v1 Hnin1 Hnin2 Hnth Hget'. 
-        edestruct Henv as [v' [Hnth'' Hcc'']]; eauto.
-        intros Hc. now inv Hc.
-        intros Hc. now inv Hc.
-        erewrite <- def_funs_neq.
-        erewrite setlist_not_In. eassumption.
-        now eauto. now eauto. now eauto.
-        eexists; eauto. split. eassumption.
-        eapply cc_approx_val_monotonic. eassumption. omega.
-  - do 3 eexists.
-    rewrite def_funs_neq. rewrite M.gss. split; eauto.
-    intros. inv H0. inv Hcc'. simpl. eauto.
-Qed.
 
-(* Fixpoint ctx_as_env (rho : env) v C : env := *)
-(*   match C with *)
-(*     | Hole_c => rho *)
-(*     | Econstr_c x tau t [f; env] C => *)
-(*       match M.get f rho with *)
-(*         | Some v1 => *)
-(*           ctx_as_env (M.set x (Vconstr tau t [v1; v]) rho) v C *)
-(*         | _ => ctx_as_env rho v C *)
-(*       end *)
-(*     | _ => rho *)
-(*   end. *)
-
-(* Lemma ctx_as_env_comp_ctx_f rho v C1 C2: *)
-(*   ctx_as_env rho v (comp_ctx_f C1 C2) = *)
-(*   ctx_as_env (ctx_as_env rho v C1) v C2. *)
-(* Admitted. *)
-(*   (* Proof. *) *)
-(* (*   revert rho. induction C1; intros rho; simpl. *) *)
-(* (*   - reflexivity. *) *)
-(* (*   - rewrite IHC1 with (rho := . Focus 3.   *) *)
-
-(* Lemma ctx_as_env_comp_ctx_f_Econstr Γ v x v' tau t B B' rho C : *)
-(*   Γ <> x -> *)
-(*   ctx_as_env *)
-(*     (M.set Γ v *)
-(*            (M.set x v' (def_funs B B' rho rho))) *)
-(*     v (comp_ctx_f C (Econstr_c x tau t [x; Γ] Hole_c)) = *)
-(*   M.set x (Vconstr tau t [v'; v]) *)
-(*         (ctx_as_env *)
-(*            (M.set Γ v *)
-(*                   (M.set x v' (def_funs B B' rho rho))) *)
-(*            v C). *)
-(* Proof. *)
-(*   intros Hneq. rewrite ctx_as_env_comp_ctx_f. simpl. *)
-(*   rewrite M.gso; eauto. now rewrite M.gss. *)
-(*   - rewrite IHC. *)
-
-
-Lemma env_inv_extend_In_Scope_l k rho rho' x v Scope Funs FVs Γ :
-  In var Scope x ->
-  env_inv k rho rho' Scope Funs Γ FVs ->
-  env_inv k (M.set x v rho) rho' Scope Funs Γ FVs.
-Proof.
-  intros Hin HInv. destruct HInv as [tau [t  [vs [Hget H]]]].
-  do 3 eexists; split; eauto. intros y n v' Hnin Hnin' Hnth Hget'.
-  rewrite M.gsspec in Hget'. destruct (Coqlib.peq y x); subst.
-  - contradiction. 
-  - eauto. 
-Qed.
-
-Lemma env_inv_extend_In_Scope_r k rho rho' x v Scope Funs FVs Γ :
-  In var Scope x ->
-  x <> Γ ->
-  env_inv k rho rho' Scope Funs Γ FVs ->
-  env_inv k rho (M.set x v rho') Scope Funs Γ FVs.
-Proof.
-  intros Hin Hneq HInv. destruct HInv as [tau [t  [vs [Hget H]]]].
-  do 3 eexists; split; eauto. rewrite M.gso; eauto.
-Qed.
-
-Lemma nthN_In {A} (l : list A) n v :
-  nthN l n = Some v ->
-  List.In v l.
-Proof. 
-  revert n v. induction l; intros n v Hnth.
-  - inv Hnth.
-  - destruct n. inv Hnth.
-    now constructor.
-    constructor 2. eapply IHl. eauto. 
-Qed. 
-
-Lemma env_inv_extend_not_In_FVs_l k rho rho' x v Scope Funs Γ FVs :
-  ~ List.In x FVs ->
-  env_inv k rho rho' Scope Funs Γ FVs ->
-  env_inv k (M.set x v rho) rho' Scope Funs Γ FVs.
-Proof.
-  intros Hin HInv. destruct HInv as [tau [t  [vs [Hget H]]]].
-  do 3 eexists; split; eauto. intros y n v' Hnin Hnin' Hnth Hget'.
-  rewrite M.gsspec in Hget'. destruct (Coqlib.peq y x); subst.
-  - inv Hget. eapply H; eauto.
-    eapply nthN_In in Hnth.
-    contradiction.
-  - eauto.
-Qed.
-
-Lemma env_inv_extend_r k rho rho' x v Scope Funs Γ FVs :
-  x <> Γ ->
-  env_inv k rho rho' Scope Funs Γ FVs ->
-  env_inv k rho (M.set x v rho') Scope Funs Γ FVs.
-Proof.
-  intros Hin HInv. destruct HInv as [tau [t  [vs [Hget H]]]].
-  do 3 eexists; split; eauto. 
-  rewrite M.gso; eauto. 
-Qed.
-
-Lemma env_inv_extend_Scope k rho rho' Scope Funs Γ FVs x :
-  env_inv k rho rho' Scope Funs Γ FVs ->
-  env_inv k rho rho' (Union _ (Singleton _ x) Scope) Funs Γ FVs.
-Proof.
-  intros [tau [t  [vs [Hget H]]]].
-  do 3 eexists; split; eauto. 
-  intros y N v Hnin Hnin' Hnth Hget'. eapply H; eauto.
-Qed.
-
-Lemma cc_approx_env_P_not_in_P_r P k rho rho' x v :
-  cc_approx_env_P P k rho rho' ->
-  ~ In _ P x ->
-  cc_approx_env_P P k rho (M.set x v rho').
-Proof. 
-  intros Hcc Hnin y Py v' Hget.
-  edestruct Hcc as [v'' [Hget' Happrox]]; eauto.
-  exists v''. rewrite M.gsspec.
-  destruct (Coqlib.peq y x); subst.
-  - contradiction.
-  - eauto.
-Qed.
-
+(** * Interpretation of evaluation contexts as environments *)
 
 Inductive ctx_to_rho : exp_ctx -> env -> env -> Prop :=
 | Hole_c_to_rho :
@@ -657,144 +497,10 @@ Inductive ctx_to_rho : exp_ctx -> env -> env -> Prop :=
       ctx_to_rho C (M.set y (Vconstr tau t [v2; v1]) rho) rho' ->
       ctx_to_rho (Econstr_c y tau t [x; Γ] C) rho rho'.
 
-  
-Lemma project_var_correct k rho1 rho2 rho2'
-      Scope Funs Γ FVs x x' C S S'  :
-  project_var Scope Funs Γ FVs S x x' C S' ->
-  cc_approx_env_P Scope k rho1 rho2 ->
-  Fun_inv k rho1 rho2 Scope Funs Γ ->
-  env_inv k rho1 rho2 Scope Funs Γ FVs ->
-  ctx_to_rho C rho2 rho2' ->
-  Disjoint _ S (Union var Scope
-                      (Union var Funs
-                             (Union var (FromList FVs) (Singleton var Γ)))) ->
-  ~ In _ S' x' /\
-  cc_approx_env_P Scope k rho1 rho2' /\
-  Fun_inv k rho1 rho2' Scope Funs Γ /\
-  env_inv k rho1 rho2' Scope Funs Γ FVs /\
-  cc_approx_var_env k rho1 rho2' x x'.
-Proof.
-  intros Hproj Hcc Hfun Henv Hctx Hd.
-  inv Hproj. 
-  - inv Hctx. repeat split; eauto. intros Hc. eapply Hd; eauto.
-  - inv Hctx. inv H12.
-    repeat split; eauto.
-    + intros Hc. inv Hc. eauto.
-    + eapply cc_approx_env_P_set_not_in_P_r. eassumption.
-      constructor. intros y Hc. eapply Hd.
-      inv Hc. inv H3. eauto. 
-    + (* TODO : make lemma *)
-      edestruct Hfun as [tau' [t' [vs' [Hget Hfun']]]].
-      rewrite Hget in H10; inv H10.
-      do 3 eexists. rewrite M.gso; [ | now intros Heq; subst; eapply Hd; eauto ].
-      split; eauto. intros f v Hnin Hin Hget''.
-      edestruct Hfun' as
-          [rhof1 [B1 [f1 [rhof2 [B2 [f2 [tau'' [t'' [Heq [Hget' Hcc']]]]]]]]]]; eauto.
-      subst. repeat eexists; eauto.
-      rewrite M.gso. eassumption. 
-      intros Hc. subst; eapply Hd; eauto.
-    + eapply env_inv_extend_r. now intros Heq; subst; eapply Hd; eauto.
-      eassumption.
-    + intros v Hget. eexists. rewrite M.gss. split; eauto.
-      edestruct Hfun as [tau' [t' [vs' [Hget' Hfun']]]].
-      rewrite Hget' in H10; inv H10.
-      edestruct Hfun' as
-          [rhof1 [B1 [f1 [rhof2 [B2 [f2 [tau'' [t'' [Heq [Hget'' Hcc']]]]]]]]]]; eauto.
-      subst. rewrite Hget'' in H11. inv H11.
-      now rewrite cc_approx_val_eq in *.
-  - inv Hctx. inv H12.
-    repeat split; eauto.
-    + intros Hc. inv Hc. eauto.
-    + eapply cc_approx_env_P_set_not_in_P_r. eassumption.
-      constructor. intros y Hc. eapply Hd.
-      inv Hc. inv H4. eauto. 
-    + edestruct Hfun as [tau' [t' [vs' [Hget Hfun']]]].
-      rewrite Hget in H10; inv H10.
-      do 3 eexists. rewrite M.gso; [ | now intros Heq; subst; eapply Hd; eauto ].
-      split; eauto. intros f v' Hnin Hin Hget''.
-      edestruct Hfun' as
-          [rhof1 [B1 [f1 [rhof2 [B2 [f2 [tau'' [t'' [Heq [Hget' Hcc']]]]]]]]]]; eauto.
-      subst. repeat eexists; eauto.
-      rewrite M.gso. eassumption. 
-      intros Hc. subst; eapply Hd; eauto.
-    + eapply env_inv_extend_r. now intros Heq; subst; eapply Hd; eauto.
-      eassumption.
-    + intros v' Hget. eexists. rewrite M.gss. split; eauto.
-      edestruct Henv as [tau' [t' [vs' [Hget' Henv']]]].
-      rewrite Hget' in H10; inv H10.
-      edestruct Henv' as [v'' [Hnth Hcc']]; eauto.
-      rewrite H11 in Hnth. now inv Hnth.
-Qed.
 
-Lemma project_var_not_In_free_set  Scope Funs Γ FVs x x' C S S'  :
-  project_var Scope Funs Γ FVs S x x' C S' ->
-  Disjoint _ S (Union var Scope
-                      (Union var Funs
-                             (Union var (FromList FVs) (Singleton var Γ)))) ->
-  ~ In _ S' x'.
-Proof.
-  intros Hproj Hd. inv Hproj; intros Hc.
-  - eapply Hd. eauto.
-  - inv Hc. exfalso. eauto.
-  - inv Hc. exfalso. eauto.    
-Qed.
+(** * Lemmas about [ctx_to_rho] *)
 
-Lemma project_var_free_set_Included Scope Funs Γ FVs x x' C S S' :
-  project_var Scope Funs Γ FVs S x x' C S' ->
-  Included _ S' S.
-Proof.
-  intros Hproj. inv Hproj.
-  - now apply Included_refl.
-  - now apply Subset_Setminus.
-  - now apply Subset_Setminus.
-Qed.
-
-Lemma project_vars_free_set_Included Scope Funs Γ FVs xs xs' C S S' :
-  project_vars Scope Funs Γ FVs S xs xs' C S' ->
-  Included _ S' S.
-Proof.
-  intros Hproj. induction Hproj.
-  - now apply Included_refl.
-  - eapply Included_trans. eassumption.
-    eapply project_var_free_set_Included. eassumption. 
-Qed.
-
-Lemma project_vars_not_In_free_set  Scope Funs Γ FVs xs xs' C S S'  :
-  project_vars Scope Funs Γ FVs S xs xs' C S' ->
-  Disjoint _ S (Union var Scope
-                      (Union var Funs
-                             (Union var (FromList FVs) (Singleton var Γ)))) ->
-  Disjoint _ S' (FromList xs').
-Proof.
-  intros Hproj Hd. induction Hproj.
-  - constructor.  intros x Hc. inv Hc. rewrite FromList_nil in H0.
-    eapply not_In_Empty_set. eassumption. 
-  - rewrite FromList_cons. eapply Disjoint_sym.
-    eapply Disjoint_Union.
-    + eapply Disjoint_sym. eapply Disjoint_Included_l.
-      eapply project_vars_free_set_Included. eassumption.
-      eapply Disjoint_Singleton.
-      eapply project_var_not_In_free_set; eassumption. 
-    + eapply Disjoint_sym. eapply IHHproj.
-      eapply Disjoint_Included_l.
-      eapply project_var_free_set_Included. eassumption.
-      eassumption.
-Qed.
-
-Lemma getlist_set_neq {A} xs x (v : A) rho :
-  ~ List.In x xs ->
-  getlist xs (M.set x v rho) = getlist xs rho. 
-Proof.
-  intros Hin.
-  revert rho. induction xs; intros rho.
-  - reflexivity.
-  - simpl. rewrite M.gso.
-    + rewrite IHxs. reflexivity.
-      intros Hin'. eapply Hin. now constructor 2.
-    + intros Heq; subst. eapply Hin. now constructor.
-Qed.
-
-Lemma ctx_to_rho_comp_ctx C C1 C2 rho rho' :
+Lemma ctx_to_rho_comp_ctx_l C C1 C2 rho rho' :
   ctx_to_rho C rho rho' ->
   comp_ctx C1 C2 C ->
   exists rho'',
@@ -822,7 +528,7 @@ Proof.
       eassumption.
 Qed.
 
-Lemma ctx_to_rho_comp_ctx_f C1 C2 rho1 rho2 rho3 :
+Lemma ctx_to_rho_comp_ctx_f_r C1 C2 rho1 rho2 rho3 :
   ctx_to_rho C1 rho1 rho2 ->
   ctx_to_rho C2 rho2 rho3 ->
   ctx_to_rho (comp_ctx_f C1 C2) rho1 rho3.
@@ -834,6 +540,112 @@ Proof.
   - simpl; econstructor; eauto.
 Qed.
 
+(** [(e1, ρ1) < (C [ e2 ], ρ2)] if [(e1, ρ1) < (e2, ρ2')], where [ρ2'] is the
+    interpretation of [C] in [ρ2] *)
+Lemma ctx_to_rho_cc_approx_exp k rho1 rho2 rho2' C e e' :
+  ctx_to_rho C rho2 rho2' ->
+  cc_approx_exp k (e, rho1) (e', rho2') ->
+  cc_approx_exp k (e, rho1) (C |[ e' ]|, rho2).
+Proof.  
+  intros Hctx Hcc. induction Hctx.
+  - assumption.
+  - intros v1 c1 Hleq1 Hstep1.
+    edestruct IHHctx as [v2 [c2 [Hstep2 Hcc2]]]; eauto.
+    repeat eexists; eauto.
+    simpl. econstructor; eauto.
+  - intros v1' c1 Hleq1 Hstep1.
+    edestruct IHHctx as [v2' [c2 [Hstep2 Hcc2]]]; eauto.
+    repeat eexists; eauto.
+    simpl. econstructor; eauto. simpl.
+    rewrite H, H0. reflexivity.
+Qed.
+
+(** * Various lemmas about [Closure_conversion_fundefs] *)
+
+Lemma closure_conversion_fundefs_find_def Funs FVs B1 B2 f t1 xs e1 :
+  Closure_conversion_fundefs Funs FVs B1 B2 ->
+  find_def f B1 = Some (t1, xs, e1) ->
+  exists t2 Γ' e2,
+    ~ In var (Union var Funs (Union _ (FromList xs) (bound_var e1))) Γ' /\
+    find_def f B2 = Some (t2, Γ' :: xs, e2) /\
+    Closure_conversion (FromList xs) Funs Γ' FVs e1 e2.
+Proof.
+  intros Hcc Hdef. induction Hcc.
+  - simpl in Hdef. destruct (M.elt_eq f f0) eqn:Heq; subst.
+    + inv Hdef. repeat eexists; eauto.
+      simpl. rewrite Heq. reflexivity.
+    + edestruct IHHcc as [t2 [Γ'' [e2 [Hnin [Hfind Hcc']]]]]; eauto.
+      repeat eexists; eauto. simpl; rewrite Heq. eassumption.
+  - inv Hdef.
+Qed.
+
+Lemma Closure_conversion_fundefs_name_in_fundefs Funs FVs B1 B2  :
+  Closure_conversion_fundefs Funs FVs B1 B2 ->
+  Same_set _ (name_in_fundefs B1) (name_in_fundefs B2).
+Proof.
+  intros Hcc. induction Hcc; simpl.
+  - eapply Same_set_Union_compat.
+    now eapply Same_set_refl.
+    now eauto.
+  - now apply Same_set_refl.
+Qed.
+
+(** * Lemmas about [project_var] and [project_vars] *)
+
+Lemma project_var_free_set_Included Scope Funs Γ FVs x x' C S S' :
+  project_var Scope Funs Γ FVs S x x' C S' ->
+  Included _ S' S.
+Proof.
+  intros Hproj. inv Hproj.
+  - now apply Included_refl.
+  - now apply Subset_Setminus.
+  - now apply Subset_Setminus.
+Qed.
+
+Lemma project_vars_free_set_Included Scope Funs Γ FVs xs xs' C S S' :
+  project_vars Scope Funs Γ FVs S xs xs' C S' ->
+  Included _ S' S.
+Proof.
+  intros Hproj. induction Hproj.
+  - now apply Included_refl.
+  - eapply Included_trans. eassumption.
+    eapply project_var_free_set_Included. eassumption. 
+Qed.
+
+Lemma project_var_not_In_free_set  Scope Funs Γ FVs x x' C S S'  :
+  project_var Scope Funs Γ FVs S x x' C S' ->
+  Disjoint _ S (Union var Scope
+                      (Union var Funs
+                             (Union var (FromList FVs) (Singleton var Γ)))) ->
+  ~ In _ S' x'.
+Proof.
+  intros Hproj Hd. inv Hproj; intros Hc.
+  - eapply Hd. eauto.
+  - inv Hc. exfalso. eauto.
+  - inv Hc. exfalso. eauto.    
+Qed.
+
+Lemma project_vars_not_In_free_set  Scope Funs Γ FVs xs xs' C S S'  :
+  project_vars Scope Funs Γ FVs S xs xs' C S' ->
+  Disjoint _ S (Union var Scope
+                      (Union var Funs
+                             (Union var (FromList FVs) (Singleton var Γ)))) ->
+  Disjoint _ S' (FromList xs').
+Proof.
+  intros Hproj Hd. induction Hproj.
+  - constructor.  intros x Hc. inv Hc. rewrite FromList_nil in H0.
+    eapply not_In_Empty_set. eassumption. 
+  - rewrite FromList_cons. eapply Disjoint_sym.
+    eapply Disjoint_Union.
+    + eapply Disjoint_sym. eapply Disjoint_Included_l.
+      eapply project_vars_free_set_Included. eassumption.
+      eapply Disjoint_Singleton.
+      eapply project_var_not_In_free_set; eassumption. 
+    + eapply Disjoint_sym. eapply IHHproj.
+      eapply Disjoint_Included_l.
+      eapply project_var_free_set_Included. eassumption.
+      eassumption.
+Qed.
 
 Lemma project_var_get Scope Funs Γ FVs S1 x x' C1 S2 rho1 rho2 y:
   project_var Scope Funs Γ FVs S1 x x' C1 S2 ->
@@ -863,7 +675,7 @@ Proof.
   induction xs; intros Scope Funs Γ FVs S1 xs' C1 S2 rho1 rho2 y Hproj Hctx Hnin.
   - inv Hproj. inv Hctx. reflexivity.
   - inv Hproj.  
-    edestruct ctx_to_rho_comp_ctx as [rho'' [Hctx1 Hctx2]]; eauto.
+    edestruct ctx_to_rho_comp_ctx_l as [rho'' [Hctx1 Hctx2]]; eauto.
     rewrite <- comp_ctx_f_correct. reflexivity.
     eapply project_var_get in Hctx1; eauto. 
     eapply IHxs in Hctx2; eauto.
@@ -906,80 +718,6 @@ Proof.
     intros Hc. eapply Hnin. eauto.
 Qed.        
 
-Lemma project_vars_correct k rho1 rho2 rho2'
-      Scope Funs Γ FVs xs xs' C S S'  :
-  project_vars Scope Funs Γ FVs S xs xs' C S' ->
-  cc_approx_env_P Scope k rho1 rho2 ->
-  Fun_inv k rho1 rho2 Scope Funs Γ ->
-  env_inv k rho1 rho2 Scope Funs Γ FVs ->
-  ctx_to_rho C rho2 rho2' ->
-  Disjoint _ S (Union var Scope
-                      (Union var Funs
-                             (Union var (FromList FVs) (Singleton var Γ)))) ->
-  cc_approx_env_P Scope k rho1 rho2' /\
-  Fun_inv k rho1 rho2' Scope Funs Γ /\
-  env_inv k rho1 rho2' Scope Funs Γ FVs /\
-  (forall vs,
-     getlist xs rho1 = Some vs ->
-     exists vs', getlist xs' rho2' = Some vs' /\
-            Forall2 (cc_approx_val k) vs vs').
-Proof.
-  revert k rho1 rho2 rho2' Scope Funs Γ FVs xs' C S.
-  induction xs;
-    intros k rho1 rho2 rho2' Scope Funs Γ FVs xs' C S Hproj Hcc Hfun Henv Hctx Hd.
-  - inv Hproj. inv Hctx. repeat split; eauto. 
-    eexists. split. reflexivity. 
-    inv H. now constructor. 
-  - inv Hproj.
-    edestruct ctx_to_rho_comp_ctx as [rho'' [Hctx1 Hctx2]]; eauto.
-    rewrite <- comp_ctx_f_correct. reflexivity.
-    eapply project_var_correct in Hctx1; eauto.
-    destruct Hctx1 as [Hnin [Hcc1 [Hfun1 [Henv1 Hcc_var]]]].
-    edestruct IHxs as [Hcc2 [Hfun2 [Henv2 Hyp]]]; eauto;
-    [ eapply Disjoint_Included_l; [| eassumption ];
-      eapply project_var_free_set_Included; eassumption |].
-    repeat split; eauto. intros vs Hget. 
-    simpl in Hget. destruct (M.get a rho1) eqn:Hget'; try discriminate. 
-    destruct (getlist xs rho1) eqn:Hgetlist; try discriminate.
-    inv Hget. edestruct Hyp as [vs' [Hgetlist' Hall]]; [ reflexivity |].
-    edestruct Hcc_var as [v' [Hget''' Hcc''']]; eauto.
-    eexists. split; eauto. simpl. rewrite Hgetlist'. 
-    erewrite <- project_vars_get; eauto. rewrite Hget'''. reflexivity.
-Qed.
-
-Lemma ctx_to_rho_cc_approx_exp k rho1 rho2 rho2' C e e' :
-  ctx_to_rho C rho2 rho2' ->
-  cc_approx_exp k (e, rho1) (e', rho2') ->
-  cc_approx_exp k (e, rho1) (C |[ e' ]|, rho2).
-Proof.  
-  intros Hctx Hcc. induction Hctx.
-  - assumption.
-  - intros v1 c1 Hleq1 Hstep1.
-    edestruct IHHctx as [v2 [c2 [Hstep2 Hcc2]]]; eauto.
-    repeat eexists; eauto.
-    simpl. econstructor; eauto.
-  - intros v1' c1 Hleq1 Hstep1.
-    edestruct IHHctx as [v2' [c2 [Hstep2 Hcc2]]]; eauto.
-    repeat eexists; eauto.
-    simpl. econstructor; eauto. simpl.
-    rewrite H, H0. reflexivity.
-Qed.
-
-Lemma Union_Included {A} S1 S2 S :
-  Included A S1 S ->
-  Included A S2 S ->
-  Included A (Union A S1 S2) S.
-Proof. 
-  intros H1 H2 x Hin; inv Hin; eauto.
-Qed.
-
-Lemma Singleton_Included {A} x S :
-  In A S x ->
-  Included A (Singleton A x) S.
-Proof. 
-  intros H x' Hin; inv Hin; eauto.
-Qed.
-
 Lemma project_var_In_Union Scope Funs Γ FVs S x x' C S' :
   project_var Scope Funs Γ FVs S x x' C S' ->
   In _ (Union var Scope (Union var Funs (FromList FVs))) x.
@@ -998,24 +736,6 @@ Proof.
     eapply Union_Included; [| eassumption ].
     eapply Singleton_Included. eapply project_var_In_Union.
     eassumption.
-Qed.
-
-Lemma project_var_ctx_to_rho Scope Funs Γ FVs x x' C S S' v1 k rho1 rho2 :
-  project_var Scope Funs Γ FVs S x x' C S' ->
-  env_inv k rho1 rho2 Scope Funs Γ FVs ->
-  Fun_inv k rho1 rho2 Scope Funs Γ ->
-  M.get x rho1 = Some v1 ->
-  exists rho2', ctx_to_rho C rho2 rho2'.
-Proof. 
-  intros Hproj [t' [tau' [vs' [Hget3' Henv]]]]
-         [t [tau [vs [Hget3 Hfun]]]] Hget1; inv Hproj.
-  - eexists; econstructor; eauto.
-  - edestruct Hfun as
-        [rho1' [B1 [f1 [rho2' [B2 [f2 [tau2 [t2 [Heq' [Hget2 Happrox2]]]]]]]]]]; eauto.
-    eexists; econstructor; eauto. constructor.
-  - rewrite Hget3 in Hget3'; inv Hget3'.
-    edestruct Henv as [y [Hnth Hcc]]; eauto.
-    eexists. econstructor; eauto. constructor. 
 Qed.
 
 Lemma project_var_not_In Scope Funs Γ FVs S x x' C S' :
@@ -1072,13 +792,62 @@ Proof.
       inv H3; eauto.
 Qed.
 
+(** * Lemmas about the existance of the interpretation of an evaluation context *)
+
+Lemma project_var_ctx_to_rho Scope Funs Γ FVs x x' C S S' v1 k rho1 rho2 :
+  project_var Scope Funs Γ FVs S x x' C S' ->
+  FV_inv k rho1 rho2 Scope Funs Γ FVs ->
+  Fun_inv k rho1 rho2 Scope Funs Γ ->
+  M.get x rho1 = Some v1 ->
+  exists rho2', ctx_to_rho C rho2 rho2'.
+Proof. 
+  intros Hproj [t' [tau' [vs' [Hget3' Henv]]]]
+         [t [tau [vs [Hget3 Hfun]]]] Hget1; inv Hproj.
+  - eexists; econstructor; eauto.
+  - edestruct Hfun as
+        [rho1' [B1 [f1 [rho2' [B2 [f2 [tau2 [t2 [Heq' [Hget2 Happrox2]]]]]]]]]]; eauto.
+    eexists; econstructor; eauto. constructor.
+  - rewrite Hget3 in Hget3'; inv Hget3'.
+    edestruct Henv as [y [Hnth Hcc]]; eauto.
+    eexists. econstructor; eauto. constructor. 
+Qed.
+
+Lemma make_closures_ctx_to_rho B Γ C k rho1 rho2  :
+  make_closures B Γ C ->
+  unique_functions B ->
+  ~ In _ (name_in_fundefs B) Γ ->
+  Fun_inv k rho1 rho2 (Empty_set _) (name_in_fundefs B) Γ ->
+  (forall f, In _ (name_in_fundefs B) f -> exists v, M.get f rho1 = Some v) ->
+  exists rho2', ctx_to_rho C rho2 rho2'.
+Proof. 
+  intros Hclo. revert rho1 rho2. induction Hclo; intros rho1 rho2 Hun Hnin Hfun Hyp. 
+  - eexists; constructor. 
+  - destruct (Hyp f) as [v' Hget'].
+    now left; eauto.
+    edestruct Hfun as [tau1 [t1 [vs1 [Hget1 Hfun']]]].
+    edestruct Hfun' as
+        [rho1f' [B1 [f1 [rho2f' [B2 [f2 [tau2 [t2 [Heq' [Hget2 Happrox2]]]]]]]]]]; eauto.
+    now apply not_In_Empty_set.
+    now left; eauto. inv Hun.
+    edestruct IHHclo as [rho2' Hctx]; [ eassumption | | | | now eexists; econstructor; eauto]. 
+    + intros Hc; eapply Hnin; right; eauto.
+    + eapply Fun_inv_set_not_In_Funs_r_not_Γ; [ eassumption | | ].
+      intros Hc; subst. eapply Hnin; now left. 
+      do 3 eexists; split; eauto; intros.
+      edestruct Hfun' as
+          [rho1'' [B1' [f1' [rho2'' [B2' [f2' [tau2' [t2' [Heq'' [Hget2' Happrox2']]]]]]]]]]; eauto.
+      right; eauto. 
+      subst. repeat eexists; eauto.
+    + intros. eapply Hyp. right; eauto.
+Qed.
+
 Lemma project_vars_ctx_to_rho Scope Funs Γ FVs xs xs' C S S' vs1 k rho1 rho2 :
   Disjoint _ S (Union var Scope
                       (Union var Funs
                              (Union var (FromList FVs) (Singleton var Γ)))) ->
   project_vars Scope Funs Γ FVs S xs xs' C S' ->
   Fun_inv k rho1 rho2 Scope Funs Γ ->
-  env_inv k rho1 rho2 Scope Funs Γ FVs ->
+  FV_inv k rho1 rho2 Scope Funs Γ FVs ->
   getlist xs rho1 = Some vs1 ->
   exists rho2', ctx_to_rho C rho2 rho2'.
 Proof. 
@@ -1119,38 +888,224 @@ Proof.
       intros Hin'. eapply HD. eauto.
     + erewrite <- project_var_get; eauto. 
       intros Hin. eapply HD. eauto.
-    + exists rho2''. eapply ctx_to_rho_comp_ctx_f; eassumption.
+    + exists rho2''. eapply ctx_to_rho_comp_ctx_f_r; eassumption.
 Qed.
 
-(* Lemma bstep_e_ctx_app rho C e1 e2 v c : *)
-(*   (forall rho v c, bstep_e rho e1 v c -> bstep_e rho e2 v c) -> *)
-(*   bstep_e rho (C |[ e1 ]|) v c-> *)
-(*   bstep_e rho (C |[ e2 ]|) v c. *)
-(* Proof.   *)
-(*   revert rho e1 e2 v c. *)
-(*   induction C; eauto; intros rho e1 e2 v' c Hyp Hstep; inv Hstep; try (now econstructor; eauto). *)
-(*   - apply findtag_append_spec in H3. *)
-(*     edestruct H3 as [Hfind | [Hfind Hnin]]. *)
-(*     + simpl. econstructor; eauto. *)
-(*       now eapply findtag_append_Some.  *)
-(*     + simpl in Hfind. edestruct (M.elt_eq t t0) eqn:Heq; subst. *)
-(*       * inv Hfind. simpl; econstructor; [| | eapply IHC ]; eauto. *)
-(*         rewrite findtag_append_not_In; [| eassumption ]. *)
-(*         simpl; now rewrite Heq. *)
-(*       * inv Hfind. simpl; econstructor; eauto. *)
-(*         rewrite findtag_append_not_In; [| eassumption ]. *)
-(*         simpl; now rewrite Heq. *)
-(*   - admit. *)
-(* Admitted. *)
+(** * Correctness lemmas *)
 
-Lemma Complement_Disjoint {A} S1 S2 :
-  Included A S1 S2 ->
-  Disjoint A (Complement _ S2) S1.
-Proof.   
-  intros Hin. constructor. intros x Hin'.
-  inv Hin'. eauto.
+(** Correctness of [closure_conversion_fundefs]. Basically un-nesting the nested
+    induction that is required by the correctness of [Closure_conversion] *) 
+Lemma Closure_conversion_fundefs_correct k rho rho' B1 B2 B1' B2'
+      Scope Γ FVs Funs' FVs' t tau vs:
+  (* The IH *)
+  (forall m : nat,
+     m < k ->
+     forall (e : exp) (rho rho' : env) (e' : exp)
+       (Scope Funs : Ensemble var) (Γ : var) (FVs : list M.elt),
+       cc_approx_env_P Scope m rho rho' ->
+       ~ In var (bound_var e) Γ ->
+       vars_in_env (occurs_free e) rho ->
+       fundefs_names_unique e ->
+       Fun_inv m rho rho' Scope Funs Γ ->
+       FV_inv m rho rho' Scope Funs Γ FVs ->
+       Closure_conversion Scope Funs Γ FVs e e' ->
+       cc_approx_exp m (e, rho) (e', rho')) ->
+  Same_set _ (occurs_free_fundefs B1) (FromList FVs) ->
+  fundefs_names_unique_fundefs B1 ->
+  vars_in_env (occurs_free_fundefs B1) rho ->
+  Closure_conversion_fundefs (name_in_fundefs B1) FVs B1 B2 ->
+  Closure_conversion_fundefs Funs' FVs' B1' B2' ->
+  ~ In _ (name_in_fundefs B1) Γ ->
+  ~ In _ (name_in_fundefs B1') Γ ->
+  closure_env k rho (Empty_set _) (Empty_set _) vs FVs ->
+  Fun_inv k (def_funs B1 B1' rho rho)
+          (def_funs B2 B2' (M.set Γ (Vconstr tau t vs) rho') (M.set Γ (Vconstr tau t vs) rho'))
+          Scope (name_in_fundefs B1') Γ.
+Proof.
+  revert B1' rho rho' B2 B1 B2' Scope Γ FVs Funs' FVs' t tau vs.
+  induction k as [k IHk] using lt_wf_rec1.
+  induction B1'; 
+    intros rho rho' B2 B1 B2' Scope Γ FVs Funs' FVs' t' tau' vs
+           IHe Hs Hun Hfv Hcc Hcc' Hnin Hnin' Henv.
+  - inv Hcc'. simpl.
+    eapply Fun_inv_set.
+    + eapply IHB1'; eauto.
+      intros Hc. apply Hnin'. simpl; eauto.
+    + intros Hc. apply Hnin'. subst. simpl; eauto.
+    + rewrite def_funs_neq.
+      rewrite M.gss. reflexivity.
+      simpl in Hnin'.
+      rewrite Closure_conversion_fundefs_name_in_fundefs in Hnin';
+        [now eauto | eassumption ].
+    + exists tau', t.
+      rewrite cc_approx_val_eq.
+      intros vs1 vs2 j t1 xs1 e1 rho1' Hlen Hfind Hset.
+      edestruct setlist_length
+      with (rho' := def_funs B2 B2 (M.set Γ (Vconstr tau' t' vs) rho')
+                             (M.set Γ (Vconstr tau' t' vs) rho')) as [rho2' Hset'].
+      eassumption. now eauto.
+      edestruct closure_conversion_fundefs_find_def
+        as [t2 [Γ'' [e2 [Hnin'' [Hfind' Hcc']]]]]; [| eassumption |]. eassumption.
+      exists t2, Γ'', xs1. do 2 eexists.
+      split. eassumption. split.
+      simpl. rewrite Hset'. reflexivity.
+      intros Hlt Hall. eapply IHe; try eassumption.  
+      * eapply cc_approx_env_P_set_not_in_P_r.
+        eapply cc_approx_env_P_setlist_l with (P1 := Empty_set _); eauto. 
+        eapply cc_approx_env_Empty_set.
+        intros x H1 H2. contradiction. now intros Hc; eauto.
+      * intros Hc. apply Hnin''. eauto.
+      * eapply vars_in_env_antimon.
+        eapply occurs_free_in_fun. eapply find_def_correct. eassumption.
+        eapply vars_in_env_setlist; [| now eauto ].
+        eapply vars_in_env_def_funs. eassumption.
+      * intros B Hin. eapply Hun. left. 
+        eapply fun_in_fundefs_funs_in_fundef; eauto.
+        eapply find_def_correct. eassumption.
+      * assert
+          (Fun_inv j (def_funs B1 B1 rho rho)
+                   (def_funs B2 B2 (M.set Γ (Vconstr tau' t' vs) rho')
+                             (M.set Γ (Vconstr tau' t' vs) rho'))
+                   (FromList xs1) (name_in_fundefs B1) Γ).
+        { eapply IHk; try eassumption.
+          - intros. eapply IHe; eauto. omega. 
+          - intros x1 N v1 Hnin1 Hnin2 Hnth Hget.
+            edestruct Henv as [v2 [Hnth' Happ']]; eauto.
+            eexists; split; eauto. eapply cc_approx_val_monotonic.
+            eassumption. omega. } 
+        eapply Fun_inv_rename with (Γ := Γ); eauto.
+        eapply Fun_inv_setlist_In_Scope_l; [ now apply Included_refl | |].
+        eapply Fun_inv_setlist_In_Scope_r; [ now apply Included_refl | |]. 
+        eapply Fun_inv_reset; [| eassumption ].
+        rewrite <- Closure_conversion_fundefs_name_in_fundefs; [ | eassumption ].
+        now eauto. now eauto. now eauto.
+      * do 3 eexists. split.
+        rewrite M.gss. reflexivity.
+        intros x N v1 Hnin1 Hnin2 Hnth Hget'. 
+        edestruct Henv as [v' [Hnth'' Hcc'']]; eauto.
+        intros Hc. now inv Hc.
+        intros Hc. now inv Hc.
+        erewrite <- def_funs_neq.
+        erewrite setlist_not_In. eassumption.
+        now eauto. now eauto. now eauto.
+        eexists; eauto. split. eassumption.
+        eapply cc_approx_val_monotonic. eassumption. omega.
+  - do 3 eexists.
+    rewrite def_funs_neq. rewrite M.gss. split; eauto.
+    intros. inv H0. inv Hcc'. simpl. eauto.
 Qed.
 
+(** Correctness of [project_var] *)
+Lemma project_var_correct k rho1 rho2 rho2'
+      Scope Funs Γ FVs x x' C S S'  :
+  project_var Scope Funs Γ FVs S x x' C S' ->
+  cc_approx_env_P Scope k rho1 rho2 ->
+  Fun_inv k rho1 rho2 Scope Funs Γ ->
+  FV_inv k rho1 rho2 Scope Funs Γ FVs ->
+  ctx_to_rho C rho2 rho2' ->
+  Disjoint _ S (Union var Scope
+                      (Union var Funs
+                             (Union var (FromList FVs) (Singleton var Γ)))) ->
+  ~ In _ S' x' /\
+  cc_approx_env_P Scope k rho1 rho2' /\
+  Fun_inv k rho1 rho2' Scope Funs Γ /\
+  FV_inv k rho1 rho2' Scope Funs Γ FVs /\
+  cc_approx_var_env k rho1 rho2' x x'.
+Proof.
+  intros Hproj Hcc Hfun Henv Hctx Hd.
+  inv Hproj. 
+  - inv Hctx. repeat split; eauto. intros Hc. eapply Hd; eauto.
+  - inv Hctx. inv H12.
+    repeat split; eauto.
+    + intros Hc. inv Hc. eauto.
+    + eapply cc_approx_env_P_set_not_in_P_r. eassumption.
+      intros Hc. eapply Hd. eauto.
+    + (* TODO : make lemma *)
+      edestruct Hfun as [tau' [t' [vs' [Hget Hfun']]]].
+      rewrite Hget in H10; inv H10.
+      do 3 eexists. rewrite M.gso; [ | now intros Heq; subst; eapply Hd; eauto ].
+      split; eauto. intros f v Hnin Hin Hget''.
+      edestruct Hfun' as
+          [rhof1 [B1 [f1 [rhof2 [B2 [f2 [tau'' [t'' [Heq [Hget' Hcc']]]]]]]]]]; eauto.
+      subst. repeat eexists; eauto.
+      rewrite M.gso. eassumption. 
+      intros Hc. subst; eapply Hd; eauto.
+    + eapply FV_inv_set_r. now intros Heq; subst; eapply Hd; eauto.
+      eassumption.
+    + intros v Hget. eexists. rewrite M.gss. split; eauto.
+      edestruct Hfun as [tau' [t' [vs' [Hget' Hfun']]]].
+      rewrite Hget' in H10; inv H10.
+      edestruct Hfun' as
+          [rhof1 [B1 [f1 [rhof2 [B2 [f2 [tau'' [t'' [Heq [Hget'' Hcc']]]]]]]]]]; eauto.
+      subst. rewrite Hget'' in H11. inv H11.
+      now rewrite cc_approx_val_eq in *.
+  - inv Hctx. inv H12.
+    repeat split; eauto.
+    + intros Hc. inv Hc. eauto.
+    + eapply cc_approx_env_P_set_not_in_P_r. eassumption.
+      intros Hc. eapply Hd. eauto.
+    + edestruct Hfun as [tau' [t' [vs' [Hget Hfun']]]].
+      rewrite Hget in H10; inv H10.
+      do 3 eexists. rewrite M.gso; [ | now intros Heq; subst; eapply Hd; eauto ].
+      split; eauto. intros f v' Hnin Hin Hget''.
+      edestruct Hfun' as
+          [rhof1 [B1 [f1 [rhof2 [B2 [f2 [tau'' [t'' [Heq [Hget' Hcc']]]]]]]]]]; eauto.
+      subst. repeat eexists; eauto.
+      rewrite M.gso. eassumption. 
+      intros Hc. subst; eapply Hd; eauto.
+    + eapply FV_inv_set_r. now intros Heq; subst; eapply Hd; eauto.
+      eassumption.
+    + intros v' Hget. eexists. rewrite M.gss. split; eauto.
+      edestruct Henv as [tau' [t' [vs' [Hget' Henv']]]].
+      rewrite Hget' in H10; inv H10.
+      edestruct Henv' as [v'' [Hnth Hcc']]; eauto.
+      rewrite H11 in Hnth. now inv Hnth.
+Qed.
+
+(** Correctness of [project_vars] *)
+Lemma project_vars_correct k rho1 rho2 rho2'
+      Scope Funs Γ FVs xs xs' C S S'  :
+  project_vars Scope Funs Γ FVs S xs xs' C S' ->
+  cc_approx_env_P Scope k rho1 rho2 ->
+  Fun_inv k rho1 rho2 Scope Funs Γ ->
+  FV_inv k rho1 rho2 Scope Funs Γ FVs ->
+  ctx_to_rho C rho2 rho2' ->
+  Disjoint _ S (Union var Scope
+                      (Union var Funs
+                             (Union var (FromList FVs) (Singleton var Γ)))) ->
+  cc_approx_env_P Scope k rho1 rho2' /\
+  Fun_inv k rho1 rho2' Scope Funs Γ /\
+  FV_inv k rho1 rho2' Scope Funs Γ FVs /\
+  (forall vs,
+     getlist xs rho1 = Some vs ->
+     exists vs', getlist xs' rho2' = Some vs' /\
+            Forall2 (cc_approx_val k) vs vs').
+Proof.
+  revert k rho1 rho2 rho2' Scope Funs Γ FVs xs' C S.
+  induction xs;
+    intros k rho1 rho2 rho2' Scope Funs Γ FVs xs' C S Hproj Hcc Hfun Henv Hctx Hd.
+  - inv Hproj. inv Hctx. repeat split; eauto. 
+    eexists. split. reflexivity. 
+    inv H. now constructor. 
+  - inv Hproj.
+    edestruct ctx_to_rho_comp_ctx_l as [rho'' [Hctx1 Hctx2]]; eauto.
+    rewrite <- comp_ctx_f_correct. reflexivity.
+    eapply project_var_correct in Hctx1; eauto.
+    destruct Hctx1 as [Hnin [Hcc1 [Hfun1 [Henv1 Hcc_var]]]].
+    edestruct IHxs as [Hcc2 [Hfun2 [Henv2 Hyp]]]; eauto;
+    [ eapply Disjoint_Included_l; [| eassumption ];
+      eapply project_var_free_set_Included; eassumption |].
+    repeat split; eauto. intros vs Hget. 
+    simpl in Hget. destruct (M.get a rho1) eqn:Hget'; try discriminate. 
+    destruct (getlist xs rho1) eqn:Hgetlist; try discriminate.
+    inv Hget. edestruct Hyp as [vs' [Hgetlist' Hall]]; [ reflexivity |].
+    edestruct Hcc_var as [v' [Hget''' Hcc''']]; eauto.
+    eexists. split; eauto. simpl. rewrite Hgetlist'. 
+    erewrite <- project_vars_get; eauto. rewrite Hget'''. reflexivity.
+Qed.
+
+
+(** Correctness of [make_closures] *)
 Lemma make_closures_correct k rho1 rho2 rho2' B Scope Funs FVs Γ Γ' C :
   make_closures B Γ' C ->
   unique_functions B ->
@@ -1159,12 +1114,12 @@ Lemma make_closures_correct k rho1 rho2 rho2' B Scope Funs FVs Γ Γ' C :
   Included _ (name_in_fundefs B) Scope ->
   cc_approx_env_P (Setminus _ Scope (name_in_fundefs B)) k rho1 rho2 ->
   Fun_inv k rho1 rho2 Scope Funs Γ ->  
-  env_inv k rho1 rho2 Scope Funs Γ FVs ->
+  FV_inv k rho1 rho2 Scope Funs Γ FVs ->
   Fun_inv k rho1 rho2 (Empty_set _) (name_in_fundefs B) Γ' ->
   ctx_to_rho C rho2 rho2' ->
   cc_approx_env_P Scope k rho1 rho2' /\
   Fun_inv k rho1 rho2' Scope Funs Γ /\
-  env_inv k rho1 rho2' Scope Funs Γ FVs.
+  FV_inv k rho1 rho2' Scope Funs Γ FVs.
 Proof.
   intros Hmake. revert k rho1 rho2 rho2' Scope Funs FVs Γ.
   induction Hmake;
@@ -1173,10 +1128,9 @@ Proof.
   - inv Hctx. repeat split; eauto.
     simpl in *.
     now rewrite Setminus_Empty_set_Same_set in Hcc. 
-  - eapply ctx_to_rho_comp_ctx in Hctx; [| apply Constr_cc; constructor ].
+  - eapply ctx_to_rho_comp_ctx_l in Hctx; [| apply Constr_cc; constructor ].
     destruct Hctx as [rho2'' [Hctx1 Hctx2]].
     inv Hctx1. inv H9. inv Hun.
-    (* destruct Hfun as [tau1 [t1 [vs [Hget Hfun]]]]. *)
     edestruct IHHmake as [Hcc1 [Hfun1 Henv1]];
       [ eassumption | | | | | | | | eassumption | ].
     + intros Hc. eapply Hnin1. right. now apply Hc. 
@@ -1187,7 +1141,7 @@ Proof.
       [| now apply (@Included_Union_Setminus _ _ (Singleton var f) _) ].
       rewrite Setminus_Union, (Union_sym (name_in_fundefs B)).
       eapply cc_approx_env_P_union.
-      eapply cc_approx_env_P_not_in_P_r. eassumption.
+      eapply cc_approx_env_P_set_not_in_P_r. eassumption.
       intros Hc. inv Hc. now eauto.
       intros f' Hs v Hget'. inv Hs.
       edestruct Hfun' as [tau2 [t2 [vs2 [Hget2 Hfun2]]]]. 
@@ -1201,7 +1155,7 @@ Proof.
     + eapply Fun_inv_set_In_Scope_r_not_Γ ; [| | eassumption ].
       * eapply Hsub. now left. 
       * intros Hc; subst. eapply Hnin1. left; eauto.
-    + eapply env_inv_extend_r; [| eassumption ].
+    + eapply FV_inv_set_r; [| eassumption ].
       intros Hc; subst. eapply Hnin1. left; eauto.
     + edestruct Hfun' as [tau2 [t2 [vs2 [Hget2 Hfun2]]]]. 
       do 3 eexists; split; eauto.
@@ -1217,172 +1171,22 @@ Proof.
     + eauto.
 Qed. 
 
-Lemma make_closures_ctx_to_rho B Γ C k rho1 rho2  :
-  make_closures B Γ C ->
-  unique_functions B ->
-  ~ In _ (name_in_fundefs B) Γ ->
-  Fun_inv k rho1 rho2 (Empty_set _) (name_in_fundefs B) Γ ->
-  (forall f, In _ (name_in_fundefs B) f -> exists v, M.get f rho1 = Some v) ->
-  exists rho2', ctx_to_rho C rho2 rho2'.
-Proof. 
-  intros Hclo. revert rho1 rho2. induction Hclo; intros rho1 rho2 Hun Hnin Hfun Hyp. 
-  - eexists; constructor. 
-  - destruct (Hyp f) as [v' Hget'].
-    now left; eauto.
-    edestruct Hfun as [tau1 [t1 [vs1 [Hget1 Hfun']]]].
-    edestruct Hfun' as
-        [rho1f' [B1 [f1 [rho2f' [B2 [f2 [tau2 [t2 [Heq' [Hget2 Happrox2]]]]]]]]]]; eauto.
-    now apply not_In_Empty_set.
-    now left; eauto. inv Hun.
-    edestruct IHHclo as [rho2' Hctx]; [ eassumption | | | | now eexists; econstructor; eauto]. 
-    + intros Hc; eapply Hnin; right; eauto.
-    + eapply Fun_inv_set_not_In_Funs_r_not_Γ; [ eassumption | | ].
-      intros Hc; subst. eapply Hnin; now left. 
-      do 3 eexists; split; eauto; intros.
-      edestruct Hfun' as
-          [rho1'' [B1' [f1' [rho2'' [B2' [f2' [tau2' [t2' [Heq'' [Hget2' Happrox2']]]]]]]]]]; eauto.
-      right; eauto. 
-      subst. repeat eexists; eauto.
-    + intros. eapply Hyp. right; eauto.
-Qed.
 
-Lemma getlist_nth_get (xs : list var) (vs : list val) rho (x : var) N :
-  getlist xs rho = Some vs ->
-  nthN xs N = Some x ->
-  exists v, nthN vs N = Some v /\ M.get x rho = Some v. 
-Proof.
-  revert vs N; induction xs; intros vs N Hget Hnth.
-  - inv Hnth. 
-  - simpl in Hget.
-    destruct (M.get a rho) eqn:Hget'; try discriminate.
-    destruct (getlist xs rho) eqn:Hgetlist'; try discriminate.
-    inv Hget. destruct N. 
-    + inv Hnth. eexists; simpl; eauto.
-    + edestruct IHxs as [v' [Hnth1 Hget1]]; eauto. 
-Qed.
-
-Lemma In_getlist (xs : list var) (rho : env) :
-  (forall x, List.In x xs -> exists v, M.get x rho = Some v) ->
-  exists vs, getlist xs rho = Some vs. 
-Proof.                                            
-  intros H. induction xs. 
-  - eexists; simpl; eauto.
-  - edestruct IHxs. 
-    + intros x Hin. eapply H. now constructor 2. 
-    + edestruct H. now constructor. 
-      eexists. simpl. erewrite H1, H0. 
-      reflexivity. 
-Qed.
-
-Lemma Fun_inv_def_funs_l k rho rho' B1 B1' Scope Funs Γ:
-  Fun_inv k rho rho' Scope Funs Γ ->
-  Fun_inv k (def_funs B1 B1' rho rho) rho'
-          (Union _ (name_in_fundefs B1')  Scope) Funs Γ.
-Proof.
-  intros [t [tau [v [Hget Hfun]]]].
-  do 3 eexists. split; eauto.
-  intros f v' Hnin Hin Hget'.
-  rewrite def_funs_neq in Hget'; eauto.
-Qed.
-
-Lemma Fun_inv_def_funs_r k rho rho' B1 B1' Scope Funs Γ:
-  ~ In _ (name_in_fundefs B1') Γ ->
-  Fun_inv k rho rho' Scope Funs Γ ->
-  Fun_inv k rho (def_funs B1 B1' rho' rho')
-          (Union _ (name_in_fundefs B1') Scope) Funs Γ.
-Proof.
-  intros Hin [t [tau [v [Hget Hfun]]]].
-  do 3 eexists. split; eauto. 
-  rewrite def_funs_neq; eauto.
-  intros f v' Hnin Hin' Hget'.
-  edestruct Hfun as
-      [rho1' [B2 [f1 [rho2' [B2' [f2 [tau2 [t2 [Heq' [Hget2 Happrox2]]]]]]]]]]; eauto.
-  repeat eexists; eauto.
-  rewrite def_funs_neq; eauto.
-Qed.
-
-Instance Fun_inv_proper :
-  Proper (Logic.eq ==> Logic.eq ==> Logic.eq ==> Same_set var ==> Logic.eq ==> Logic.eq ==> iff)
-         (Fun_inv).
-Proof.
-  constructor; subst; intros [tau [t [vs [Hget Hfun]]]]; do 3 eexists; split; eauto;
-  intros; eapply Hfun; eauto; intros Hc; eapply H; eapply H2; eauto.
-Qed.
-
-Lemma Fun_inv_def_funs k rho rho' B1 B1' B2 B2' Scope Funs Γ:
-  ~ In _ (name_in_fundefs B1') Γ ->
-  Same_set _ (name_in_fundefs B1') (name_in_fundefs B2') ->
-  Fun_inv k rho rho' Scope Funs Γ ->
-  Fun_inv k  (def_funs B1 B1' rho rho) (def_funs B2 B2' rho' rho')
-          (Union _ (name_in_fundefs B1') Scope) Funs Γ.
-Proof.
-  intros Hin HS [t [tau [v [Hget Hfun]]]].
-  do 3 eexists. split; eauto. 
-  rewrite def_funs_neq; eauto.
-  intros Hc. eapply Hin. now eapply HS.
-  intros f v' Hnin Hin' Hget'.
-  rewrite def_funs_neq in Hget'; eauto.
-  edestruct Hfun as
-      [rho1' [B3 [f1 [rho2' [B3' [f2 [tau2 [t2 [Heq' [Hget2 Happrox2]]]]]]]]]]; eauto.
-  repeat eexists; eauto.
-  rewrite def_funs_neq; eauto.
-  intros Hc. eapply Hnin. left. now rewrite HS.
-Qed.
-
-Lemma cc_approx_env_P_def_funs_not_In_P_l k rho1 rho2 S B B' :
-  Disjoint _ S (name_in_fundefs B') ->
-  cc_approx_env_P S k rho1 rho2 ->
-  cc_approx_env_P S k (def_funs B B' rho1 rho1) rho2.
-Proof.
-  intros Hd Hcc x HS v Hget. eapply Hcc; eauto. 
-  erewrite <- def_funs_neq. eassumption.  
-  intros Hc. eapply Hd; constructor; eauto.
-Qed.
-
-Lemma cc_approx_env_P_def_funs_not_In_P_r k rho1 rho2 S B B' :
-  Disjoint _ S (name_in_fundefs B') ->
-  cc_approx_env_P S k rho1 rho2 ->
-  cc_approx_env_P S k rho1 (def_funs B B' rho2 rho2).
-Proof.
-  intros Hd Hcc x HS v Hget.
-  edestruct Hcc as [v' [Hget' Hcc']]; eauto.
-  eexists; split; eauto.
-  rewrite def_funs_neq. eassumption.
-  intros Hc. eapply Hd; constructor; eauto.
-Qed.
-
-Lemma env_inv_def_funs k rho rho' B1 B1' B2 B2' Scope Funs Γ FVs:
-  ~ In _ (name_in_fundefs B1') Γ ->
-  Same_set _ (name_in_fundefs B1') (name_in_fundefs B2') ->
-  env_inv k rho rho' Scope Funs Γ FVs ->
-  env_inv k  (def_funs B1 B1' rho rho) (def_funs B2 B2' rho' rho')
-          (Union _ (name_in_fundefs B1') Scope) Funs Γ FVs.
-Proof.
-  intros Hin HS [t [tau [v [Hget Henv]]]].
-  do 3 eexists. split; eauto. 
-  rewrite def_funs_neq; eauto.
-  intros Hc. eapply Hin. now eapply HS.
-  intros f N v' Hnin Hnin' Hnth Hget'.
-  rewrite def_funs_neq in Hget'; eauto.
-Qed.
-
-Corollary Fun_inv_def_funs' k rho rho' B1 B1' B2 B2' Scope Funs Γ:
-  ~ In _ (name_in_fundefs B1') Γ ->
-  Same_set _ (name_in_fundefs B1') (name_in_fundefs B2') ->
-  Fun_inv k rho rho' Scope Funs Γ ->
-  Fun_inv k  (def_funs B1 B1' rho rho) (def_funs B2 B2' rho' rho')
-          (Union _ (name_in_fundefs B2') Scope) Funs Γ.
-Proof.
-  intros Hin HS Hf. rewrite <- HS. now apply Fun_inv_def_funs.
-Qed.
-
-Lemma closure_conversion_correct k rho rho' e e' Scope Funs Γ FVs :
+(** Correctness of [Closure_conversion] *)
+Lemma Closure_conversion_correct k rho rho' e e' Scope Funs Γ FVs :
+  (* [Scope] invariant *)
   cc_approx_env_P Scope k rho rho' ->
+  (* [Γ] (the current environment parameter) is not bound in e *)
   ~ In _ (bound_var e) Γ ->
+  (* The free variables of e are defined in the environment *)
   vars_in_env (occurs_free e) rho ->
+  (* The blocks of functions have unique function names *)
   fundefs_names_unique e ->
+  (* [Fun] invariant *)
   Fun_inv k rho rho' Scope Funs Γ ->
-  env_inv k rho rho' Scope Funs Γ FVs ->
+  (* Free variables invariant *)
+  FV_inv k rho rho' Scope Funs Γ FVs ->
+  (* [e'] is the closure conversion of [e] *)
   Closure_conversion Scope Funs Γ FVs e e' ->
   cc_approx_exp k (e, rho) (e', rho').
 Proof.
@@ -1410,7 +1214,7 @@ Proof.
       eapply Setminus_Included. now apply Included_refl.
       rewrite cc_approx_val_eq. constructor; eauto.
       now eapply Forall2_Forall2_asym_included.
-    + eapply vars_in_env_antimon; [| eapply vars_in_env_extend; eassumption ].
+    + eapply vars_in_env_antimon; [| eapply vars_in_env_set; eassumption ].
       eapply occurs_free_Econstr_Included. 
     + intros f Hfin. eauto.
     + eapply Fun_inv_set_In_Scope_l. now eauto.
@@ -1418,9 +1222,9 @@ Proof.
       intros Heq; subst. now eauto.
       eapply Fun_inv_mon; [ | now eauto ].
       eapply Included_Union_r.
-    + eapply env_inv_extend_In_Scope_l. now constructor.
-      eapply env_inv_extend_r. intros Hc. eapply Hnin.
-      subst. now eauto. now eapply env_inv_extend_Scope.
+    + eapply FV_inv_set_In_Scope_l. now constructor.
+      eapply FV_inv_set_r. intros Hc. eapply Hnin.
+      subst. now eauto. now eapply FV_inv_extend_Scope.
     + repeat eexists; [| eassumption ].
       econstructor; eauto.
   - (* Case [Ecase x []] *)
@@ -1459,14 +1263,14 @@ Proof.
            | repeat eexists; [| eassumption ]; econstructor; eauto;
              econstructor; eauto;
              [ rewrite M.gss ; reflexivity | simpl; now rewrite Heq ] ].
-        + eapply cc_approx_env_P_not_in_P_r; now eauto.
+        + eapply cc_approx_env_P_set_not_in_P_r; now eauto.
         + eapply vars_in_env_antimon; [|  eassumption ].
           eapply occurs_free_Ecase_Included. now constructor.
         + intros f Hfin. eapply Hun.
           econstructor. eassumption. now constructor. 
         + eapply Fun_inv_set_not_In_Funs_r_not_Γ. now eauto.
           intros Heq'; subst. now eauto. eassumption.
-        + eapply env_inv_extend_r. intros Hc. subst. now eauto.
+        + eapply FV_inv_set_r. intros Hc. subst. now eauto.
           eassumption. }
     { inv H3. assert (H5' := H5). inv H5. 
       - edestruct Happrox as [vcon [Hget' Happrox2]]; eauto.
@@ -1523,7 +1327,7 @@ Proof.
       Setminus_Empty_set, Union_Empty_set_r. 
       eapply cc_approx_env_P_antimon; [ eassumption |].
       eapply Setminus_Included. now apply Included_refl.      
-    + eapply vars_in_env_antimon; [| eapply vars_in_env_extend; eassumption ].
+    + eapply vars_in_env_antimon; [| eapply vars_in_env_set; eassumption ].
       eapply occurs_free_Eproj_Included. 
     + intros f Hfin. eauto.
     + eapply Fun_inv_set_In_Scope_l. now eauto.
@@ -1531,9 +1335,9 @@ Proof.
       intros Heq; subst. now eauto.
       eapply Fun_inv_mon; [ | now eauto ].
       eapply Included_Union_r.
-    + eapply env_inv_extend_In_Scope_l. now constructor.
-      eapply env_inv_extend_r. intros Hc. eapply Hnin.
-      subst. now eauto. now eapply env_inv_extend_Scope.
+    + eapply FV_inv_set_In_Scope_l. now constructor.
+      eapply FV_inv_set_r. intros Hc. eapply Hnin.
+      subst. now eauto. now eapply FV_inv_extend_Scope.
     + repeat eexists; [| eassumption ].
       econstructor; eauto.
   - (* Case Efun -- the hardest one! *) 
@@ -1554,7 +1358,7 @@ Proof.
                             (C |[ e'0 ]|, def_funs B' B' (M.set Γ' (Vconstr tau t v') rho2')
                                        (M.set Γ' (Vconstr tau t v') rho2'))).
     { edestruct make_closures_ctx_to_rho as [rho2'' Htp_rho']; eauto.
-      - eapply closure_conversion_fundefs_correct; eauto.
+      - eapply Closure_conversion_fundefs_correct; eauto.
         + intros f Hfin. inv Hfin; eauto.
         + eapply vars_in_env_antimon; [| eassumption ].
           intros x H. eapply Free_Efun2. eassumption. 
@@ -1564,7 +1368,7 @@ Proof.
           now apply Hgetlist. eassumption.
           edestruct (@Forall2_nthN val) as [v'' [Hget''' Hcc'']]. eassumption.
           eassumption. rewrite Hget in Hget''. inv Hget''. eauto.
-      - intros. now eapply get_def_funs_In_names.
+      - intros f' Hin. eexists. now rewrite def_funs_eq.
       - edestruct make_closures_correct with
           (Scope := Union var (name_in_fundefs f2) Scope)
           (Γ := Γ)
@@ -1583,7 +1387,7 @@ Proof.
           eapply cc_approx_env_P_def_funs_not_In_P_r.
           eapply Disjoint_Setminus. rewrite <- Closure_conversion_fundefs_name_in_fundefs.
           now apply Included_refl. eauto.
-          eapply cc_approx_env_P_not_in_P_r.
+          eapply cc_approx_env_P_set_not_in_P_r.
           eapply cc_approx_env_P_antimon. eassumption.
           rewrite Setminus_Union_distr, Setminus_Empty_set, Union_Empty_set_r.
           eapply Setminus_Included. now apply Included_refl.
@@ -1595,14 +1399,14 @@ Proof.
           * eapply Fun_inv_set_not_In_Funs_r_not_Γ; [| | eassumption ].
             intros Hc. eapply H2. eauto.
             intros Hc. eapply H2. subst. eauto.
-        + eapply env_inv_def_funs.
+        + eapply FV_inv_def_funs.
           * intros Hc. eapply Hnin. constructor.
             now eapply name_in_fundefs_bound_var_fundefs.
           * eapply Closure_conversion_fundefs_name_in_fundefs. eassumption.
-          * eapply  env_inv_extend_r.
+          * eapply  FV_inv_set_r.
             intros Hc. eapply H2. subst. eauto.
             eassumption. 
-        + eapply closure_conversion_fundefs_correct; eauto.
+        + eapply Closure_conversion_fundefs_correct; eauto.
           * intros f Hfin. inv Hfin; eauto.
           * eapply vars_in_env_antimon; [| eassumption ].
             intros x H. eapply Free_Efun2. eassumption. 
@@ -1641,7 +1445,7 @@ Proof.
       * intros v1' c1' Hleq' Hstep'.
         inv Hstep'. rewrite H4 in H6. inv H6.
         rewrite H8 in H13; inv H13.
-        admit. (* the relation needs tweaking *)
+        admit. (* the semantics/relation needs tweaking *)
         rewrite H4 in H3. congruence.
       * constructor; eauto.
     + edestruct project_vars_ctx_to_rho as [rho2' Hto_rho]; eauto.
@@ -1708,7 +1512,7 @@ Proof.
       Setminus_Empty_set, Union_Empty_set_r. 
       eapply cc_approx_env_P_antimon; [ eassumption |].
       eapply Setminus_Included. now apply Included_refl.
-    + eapply vars_in_env_antimon; [| eapply vars_in_env_extend; eassumption ].
+    + eapply vars_in_env_antimon; [| eapply vars_in_env_set; eassumption ].
       eapply occurs_free_Eprim_Included. 
     + intros f Hfin. eauto.
     + eapply Fun_inv_set_In_Scope_l. now eauto.
@@ -1716,9 +1520,9 @@ Proof.
       intros Heq; subst. now eauto.
       eapply Fun_inv_mon; [ | now eauto ].
       eapply Included_Union_r.
-    + eapply env_inv_extend_In_Scope_l. now constructor.
-      eapply env_inv_extend_r. intros Hc. eapply Hnin.
-      subst. now eauto. now eapply env_inv_extend_Scope.
+    + eapply FV_inv_set_In_Scope_l. now constructor.
+      eapply FV_inv_set_r. intros Hc. eapply Hnin.
+      subst. now eauto. now eapply FV_inv_extend_Scope.
     + repeat eexists; [| eassumption ].
       econstructor; eauto.
 Admitted.
